Prove that normal form is unique (modulo beta/eta)
Theory Idiomatic_Terms now depends on session HOL-Proofs-Lambda.

experiments/Idiomatic_Terms.thy
@@ -1,36 +1,332 @@
 theory Idiomatic_Terms
-imports Main
+imports Lambda Eta  (* in HOL-Proofs-Lambda *)
 begin
 
 section {* Operations on idiomatic terms *}
 
-subsection {* Lambda terms *}
+subsection {* Extensions to lambda terms *}
 
-datatype 'a trm =
-    Var 'a | BVar nat
-  | Abs "'a trm"
-  | App "'a trm" "'a trm" (infixl "$" 200)
+subsubsection {* Combined beta- and eta-reduction *}
 
-abbreviation "\<B> \<equiv> Abs (Abs (Abs (BVar 2 $ (BVar 1 $ BVar 0))))"
-abbreviation "\<B>\<^sub>1 f \<equiv> Abs (Abs (f $ (BVar 1 $ BVar 0)))"
+abbreviation beta_eta :: "dB \<Rightarrow> dB \<Rightarrow> bool" (infixl "\<rightarrow>\<^sub>\<beta>\<^sub>\<eta>" 50)
+where
+  "s \<rightarrow>\<^sub>\<beta>\<^sub>\<eta> t \<equiv> s \<rightarrow>\<^sub>\<beta> t \<or> s \<rightarrow>\<^sub>\<eta> t"
+
+abbreviation beta_eta_reds :: "dB \<Rightarrow> dB \<Rightarrow> bool" (infixl "\<rightarrow>\<^sub>\<beta>\<^sub>\<eta>\<^sup>*" 50)
+where
+  "s \<rightarrow>\<^sub>\<beta>\<^sub>\<eta>\<^sup>* t \<equiv> (beta_eta)\<^sup>*\<^sup>* s t"
+
+lemma beta_eta_appl: "s \<rightarrow>\<^sub>\<beta>\<^sub>\<eta>\<^sup>* s' \<Longrightarrow> s \<degree> t \<rightarrow>\<^sub>\<beta>\<^sub>\<eta>\<^sup>* s' \<degree> t"
+by (induction set: rtranclp) (auto intro: rtranclp.rtrancl_into_rtrancl)
+
+lemma beta_eta_appr: "t \<rightarrow>\<^sub>\<beta>\<^sub>\<eta>\<^sup>* t' \<Longrightarrow> s \<degree> t \<rightarrow>\<^sub>\<beta>\<^sub>\<eta>\<^sup>* s \<degree> t'"
+by (induction set: rtranclp) (auto intro: rtranclp.rtrancl_into_rtrancl)
+
+lemma beta_eta_abs[intro]: "t \<rightarrow>\<^sub>\<beta>\<^sub>\<eta>\<^sup>* t' \<Longrightarrow> Abs t \<rightarrow>\<^sub>\<beta>\<^sub>\<eta>\<^sup>* Abs t'"
+by (induction set: rtranclp) (auto intro: rtranclp.rtrancl_into_rtrancl)
+
+lemma beta_mono: "s \<rightarrow>\<^sub>\<beta>\<^sup>* t \<Longrightarrow> s \<rightarrow>\<^sub>\<beta>\<^sub>\<eta>\<^sup>* t"
+by (auto intro: rtranclp_mono[THEN predicate2D])
+
+lemma eta_mono: "s \<rightarrow>\<^sub>\<eta>\<^sup>* t \<Longrightarrow> s \<rightarrow>\<^sub>\<beta>\<^sub>\<eta>\<^sup>* t"
+by (auto intro: rtranclp_mono[THEN predicate2D])
+
+lemma beta_eta_confluent: "confluent beta_eta"
+proof -
+  have "beta_eta = sup beta eta" by blast
+  with Eta.confluent_beta_eta show ?thesis by simp
+qed
+
+
+subsubsection {* Equivalent terms *}
+
+definition term_equiv :: "dB \<Rightarrow> dB \<Rightarrow> bool" (infixl "\<leftrightarrow>" 50)
+where
+  "s \<leftrightarrow> t = (\<exists>u. s \<rightarrow>\<^sub>\<beta>\<^sub>\<eta>\<^sup>* u \<and> t \<rightarrow>\<^sub>\<beta>\<^sub>\<eta>\<^sup>* u)"
+
+lemma term_refl[simp,intro]: "t \<leftrightarrow> t"
+unfolding term_equiv_def by blast
+
+lemma term_sym[sym]: "(s \<leftrightarrow> t) \<Longrightarrow> (t \<leftrightarrow> s)"
+unfolding term_equiv_def by blast
+
+lemma diamond_merge: "diamond P \<Longrightarrow> P x y \<Longrightarrow> P x z \<Longrightarrow> (\<exists>w. P y w \<and> P z w)"
+unfolding diamond_def commute_def square_def
+by blast
+
+lemma term_trans[trans]: "s \<leftrightarrow> t \<Longrightarrow> t \<leftrightarrow> u \<Longrightarrow> s \<leftrightarrow> u"
+proof -
+  assume "s \<leftrightarrow> t"
+  then obtain x where A: "s \<rightarrow>\<^sub>\<beta>\<^sub>\<eta>\<^sup>* x" and B: "t \<rightarrow>\<^sub>\<beta>\<^sub>\<eta>\<^sup>* x"
+    unfolding term_equiv_def by blast
+  assume "t \<leftrightarrow> u"
+  then obtain y where B': "t \<rightarrow>\<^sub>\<beta>\<^sub>\<eta>\<^sup>* y" and C: "u \<rightarrow>\<^sub>\<beta>\<^sub>\<eta>\<^sup>* y"
+    unfolding term_equiv_def by blast
+  from B B' obtain z where D: "x \<rightarrow>\<^sub>\<beta>\<^sub>\<eta>\<^sup>* z" "y \<rightarrow>\<^sub>\<beta>\<^sub>\<eta>\<^sup>* z"
+    using diamond_merge[OF beta_eta_confluent] by blast
+  from A C D show "s \<leftrightarrow> u"
+    unfolding term_equiv_def by (blast intro: rtranclp_trans)
+qed
+
+lemma term_appl: "s \<leftrightarrow> s' \<Longrightarrow> s \<degree> t \<leftrightarrow> s' \<degree> t"
+unfolding term_equiv_def
+by (blast intro: beta_eta_appl)
+
+lemma term_appr: "t \<leftrightarrow> t' \<Longrightarrow> s \<degree> t \<leftrightarrow> s \<degree> t'"
+unfolding term_equiv_def
+by (blast intro: beta_eta_appr)
+
+lemma term_abs[intro]: "t \<leftrightarrow> t' \<Longrightarrow> Abs t \<leftrightarrow> Abs t'"
+unfolding term_equiv_def
+by blast
+
+lemma beta_eta_red: "s \<rightarrow>\<^sub>\<beta>\<^sub>\<eta>\<^sup>* t \<Longrightarrow> s \<leftrightarrow> t"
+unfolding term_equiv_def
+by blast
+
+
+subsubsection {* Some combinators *}
+
+abbreviation "\<I> \<equiv> Abs (Var 0)"
+abbreviation "\<B> \<equiv> Abs (Abs (Abs (Var 2 \<degree> (Var 1 \<degree> Var 0))))"
+abbreviation "\<A>' \<equiv> Abs (Abs (Var 0 \<degree> Var 1))" -- {* reverse application *}
+
+lemma I_eval: "\<I> \<degree> x \<rightarrow>\<^sub>\<beta>\<^sup>* x"
+proof -
+  have "\<I> \<degree> x \<rightarrow>\<^sub>\<beta> x" by (metis beta.beta subst_eq)
+  thus ?thesis by simp
+qed
+
+lemmas I_equiv = I_eval[THEN beta_mono, THEN beta_eta_red]
+
+lemma subst_lift2[simp]: "(lift (lift t 0) 0)[x/Suc 0] = lift t 0"
+proof -
+  have "lift (lift t 0) 0 = lift (lift t 0) (Suc 0)" using lift_lift by simp
+  thus ?thesis by simp
+qed
+
+lemma B_eval: "\<B> \<degree> g \<degree> f \<degree> x \<rightarrow>\<^sub>\<beta>\<^sup>* g \<degree> (f \<degree> x)"
+proof -
+  have "\<B> \<degree> g \<degree> f \<degree> x \<rightarrow>\<^sub>\<beta> Abs (Abs (Var 2 \<degree> (Var 1 \<degree> Var 0)))[g/0] \<degree> f \<degree> x"
+    by clarify
+  also have "... = Abs (Abs (lift (lift g 0) 0 \<degree> (Var 1 \<degree> Var 0))) \<degree> f \<degree> x"
+    by (simp add: numerals)
+  also have "... \<rightarrow>\<^sub>\<beta>\<^sup>* Abs (lift (lift g 0) 0 \<degree> (Var 1 \<degree> Var 0))[f/0] \<degree> x"
+    by (rule r_into_rtranclp) clarify
+  also have "... = Abs (lift g 0 \<degree> (lift f 0 \<degree> Var 0)) \<degree> x"
+    by simp
+  also have "... \<rightarrow>\<^sub>\<beta>\<^sup>* (lift g 0 \<degree> (lift f 0 \<degree> Var 0))[x/0]"
+    by (rule r_into_rtranclp) clarify
+  also have "... = g \<degree> (f \<degree> x)" by simp
+  finally show ?thesis .
+qed
+
+lemmas B_equiv = B_eval[THEN beta_mono, THEN beta_eta_red]
+
+lemma A'_eval: "\<A>' \<degree> x \<degree> f \<rightarrow>\<^sub>\<beta>\<^sup>* f \<degree> x"
+proof -
+  have "\<A>' \<degree> x \<degree> f \<rightarrow>\<^sub>\<beta> Abs (Var 0 \<degree> Var 1)[x/0] \<degree> f" by clarify
+  also have "... = Abs (Var 0 \<degree> lift x 0) \<degree> f" by simp
+  also have "... \<rightarrow>\<^sub>\<beta>\<^sup>* (Var 0 \<degree> lift x 0)[f/0]" by (rule r_into_rtranclp) clarify
+  also have "... \<rightarrow>\<^sub>\<beta>\<^sup>* f \<degree> x" by simp
+  finally show ?thesis .
+qed
+
+lemmas A'_equiv = A'_eval[THEN beta_mono, THEN beta_eta_red]
+
+
+subsubsection {* Auxiliary lemmas *}
+
+lemma subst_liftn:
+  "i \<le> n + k \<and> k \<le> i \<Longrightarrow> (liftn (Suc n) s k)[t/i] = liftn n s k"
+by (induction s arbitrary: i k t) auto
+
+lemma free_liftn:
+  "free (liftn n t k) i = (i < k \<and> free t i \<or> k + n \<le> i \<and> free t (i - n))"
+proof (induction t arbitrary: k i)
+  case (Var x)
+  show ?case by simp arith
+next
+  case (App s t)
+  thus ?case by auto
+next
+  case (Abs t)
+  thus ?case by simp (metis Suc_diff_le add_leD2)
+qed
 
 
 subsection {* Idiomatic terms *}
 
-datatype 'a itrm =
-    Imp "'a trm" | Pure "'a trm"
-  | IAp "'a itrm" "'a itrm" (infixl "\<diamond>" 150)
+subsubsection {* Basic definitions *}
 
-primrec leaves :: "'a itrm \<Rightarrow> nat"
+datatype itrm =
+    Term dB | Pure dB
+  | IAp itrm itrm (infixl "\<diamond>" 150)
+
+inductive itrm_cong :: "itrm \<Rightarrow> itrm \<Rightarrow> bool" (infixl "\<cong>" 50)
+where
+    "t \<leftrightarrow> t' \<Longrightarrow> Term t \<cong> Term t'"
+  | "t \<leftrightarrow> t' \<Longrightarrow> Pure t \<cong> Pure t'"
+  | "f \<cong> f' \<Longrightarrow> f \<diamond> x \<cong> f' \<diamond> x"
+  | "x \<cong> x' \<Longrightarrow> f \<diamond> x \<cong> f \<diamond> x'"
+
+inductive itrm_equiv :: "itrm \<Rightarrow> itrm \<Rightarrow> bool" (infixl "\<simeq>" 50)
+where
+    itrm_id: "x \<simeq> Pure \<I> \<diamond> x"
+  | itrm_comp: "g \<diamond> (f \<diamond> x) \<simeq> Pure \<B> \<diamond> g \<diamond> f \<diamond> x"
+  | itrm_hom: "Pure f \<diamond> Pure x \<simeq> Pure (f \<degree> x)"
+  | itrm_xchng: "f \<diamond> Pure x \<simeq> Pure (\<A>' \<degree> x) \<diamond> f"
+  | itrm_apl: "f \<simeq> f' \<Longrightarrow> f \<diamond> x \<simeq> f' \<diamond> x"
+  | itrm_apr: "x \<simeq> x' \<Longrightarrow> f \<diamond> x \<simeq> f \<diamond> x'"
+  | itrm_refl[simp,intro]: "x \<simeq> x"
+  | itrm_sym[sym]: "x \<simeq> y \<Longrightarrow> y \<simeq> x"
+  | itrm_trans[trans]: "x \<simeq> y \<Longrightarrow> y \<simeq> z \<Longrightarrow> x \<simeq> z"
+
+
+subsubsection {* Structural analysis *}
+
+primrec opaque :: "itrm \<Rightarrow> dB list"
+where
+    "opaque (Term x) = [x]"
+  | "opaque (Pure _) = []"
+  | "opaque (f \<diamond> x) = opaque f @ opaque x"
+
+abbreviation "iorder x \<equiv> length (opaque x)"
+
+primrec vary_terms :: "nat \<Rightarrow> itrm \<Rightarrow> nat \<Rightarrow> dB \<times> nat"
+where
+    "vary_terms n (Term _) i = (Var i, Suc i)"
+  | "vary_terms n (Pure x) i = (liftn n x 0, i)"
+  | "vary_terms n (f \<diamond> x)  i = (case vary_terms n x i of (x', i') \<Rightarrow>
+        apfst (\<lambda>f. f \<degree> x') (vary_terms n f i'))"
+
+abbreviation "unlift' n x i \<equiv> fst (vary_terms n x i)"
+
+primrec wrap_abs :: "dB \<Rightarrow> nat \<Rightarrow> dB"
+where
+    "wrap_abs t 0 = t"
+  | "wrap_abs t (Suc n) = Abs (wrap_abs t n)"
+
+abbreviation "unlift x \<equiv> wrap_abs (unlift' (iorder x) x 0) (iorder x)"
+
+
+lemma vary_terms_order: "snd (vary_terms n x i) = i + iorder x"
+by (induction arbitrary: i) (auto simp add: case_prod_unfold)
+
+lemma unlift_ap: "unlift' n (f \<diamond> x) i = unlift' n f (i + iorder x) \<degree> unlift' n x i"
+by (simp add: case_prod_unfold vary_terms_order)
+
+lemma free_unlift: "free (unlift' n x i) j \<Longrightarrow> j \<ge> n \<or> (j \<ge> i \<and> j < i + iorder x)"
+proof (induction x arbitrary: i)
+  case (Term x)
+  thus ?case by simp
+next
+  case (Pure x)
+  thus ?case using free_liftn by simp
+next
+  case (IAp x y)
+  thus ?case unfolding unlift_ap by fastforce
+qed
+
+lemma unlift_subst: "j \<le> i \<and> j \<le> n \<Longrightarrow> (unlift' (Suc n) t (Suc i))[s/j] = unlift' n t i"
+proof (induction t arbitrary: i)
+  case (Term x)
+  thus ?case by simp
+next
+  case (Pure x)
+  thus ?case using subst_liftn by simp
+next
+  case (IAp x y)
+  thus ?case using unlift_ap by simp
+qed
+
+lemma wrap_abs_inside: "wrap_abs t (Suc n) = wrap_abs (Abs t) n"
+by (induction n) auto
+
+lemma wrap_abs_equiv: "s \<leftrightarrow> t \<Longrightarrow> wrap_abs s n \<leftrightarrow> wrap_abs t n"
+by (induction n) auto
+
+
+lemma opaque_equiv:
+  assumes "x \<simeq> y"
+    shows "opaque x = opaque y"
+using assms by induction auto
+
+lemma unlift'_equiv:
+  assumes "x \<simeq> y"
+    shows "unlift' n x i \<leftrightarrow> unlift' n y i"
+using assms proof (induction arbitrary: n i)
+  case (itrm_id x)
+  show ?case
+    unfolding unlift_ap using I_equiv[symmetric] by simp
+next
+  case (itrm_comp g f x)
+  let ?G = "unlift' n g (i + iorder f + iorder x)"
+  let ?F = "unlift' n f (i + iorder x)"
+  let ?X = "unlift' n x i"
+  have "unlift' n (g \<diamond> (f \<diamond> x)) i = ?G \<degree> (?F \<degree> ?X)"
+    unfolding unlift_ap by (simp add: add.assoc)
+  moreover have "unlift' n (Pure \<B> \<diamond> g \<diamond> f \<diamond> x) i = \<B> \<degree> ?G \<degree> ?F \<degree> ?X"
+    unfolding unlift_ap by (simp add: add.commute add.left_commute)
+  moreover have "?G \<degree> (?F \<degree> ?X) \<leftrightarrow> \<B> \<degree> ?G \<degree> ?F \<degree> ?X" using B_equiv[symmetric] .
+  ultimately show ?case by simp
+next
+  case (itrm_hom f x)
+  show ?case by auto
+next
+  case (itrm_xchng f x)
+  let ?F = "unlift' n f i"
+  let ?X = "liftn n x 0"
+  have "unlift' n (f \<diamond> Pure x) i = ?F \<degree> ?X"
+    unfolding unlift_ap by simp
+  moreover have "unlift' n (Pure (\<A>' \<degree> x) \<diamond> f) i = \<A>' \<degree> ?X \<degree> ?F"
+    unfolding unlift_ap by simp
+  moreover have "?F \<degree> ?X \<leftrightarrow> \<A>' \<degree> ?X \<degree> ?F" using A'_equiv[symmetric] .
+  ultimately show ?case by simp
+next
+  case (itrm_apl f f' x)
+  have "unlift' n (f \<diamond> x) i = unlift' n f (i + iorder x) \<degree> unlift' n x i"
+    unfolding unlift_ap by simp
+  moreover have "unlift' n (f' \<diamond> x) i = unlift' n f' (i + iorder x) \<degree> unlift' n x i"
+    unfolding unlift_ap by simp
+  ultimately show ?case using itrm_apl.IH term_appl by auto
+next
+  case (itrm_apr x x' f)
+  from itrm_apr.hyps have order_eq: "iorder x = iorder x'"
+    using opaque_equiv by auto
+  have "unlift' n (f \<diamond> x) i = unlift' n f (i + iorder x) \<degree> unlift' n x i"
+    unfolding unlift_ap by simp
+  moreover have "unlift' n (f \<diamond> x') i = unlift' n f (i + iorder x) \<degree> unlift' n x' i"
+    unfolding unlift_ap order_eq by simp
+  ultimately show ?case using itrm_apr.IH term_appr by auto
+next
+  case itrm_refl
+  show ?case ..
+next
+  case itrm_sym
+  thus ?case using term_sym by simp
+next
+  case itrm_trans
+  thus ?case using term_trans by blast
+qed
+
+lemma unlift_equiv:
+  assumes "x \<simeq> y"
+    shows "unlift x \<leftrightarrow> unlift y"
+using assms unlift'_equiv wrap_abs_equiv opaque_equiv
+by simp
+
+
+primrec leaves :: "itrm \<Rightarrow> nat"
 where
     "leaves (Pure _) = 1"
-  | "leaves (Imp _)  = 1"
+  | "leaves (Term _)  = 1"
   | "leaves (f \<diamond> x)  = leaves f + leaves x"
 
-primrec rleaves :: "'a itrm \<Rightarrow> nat"
+primrec rleaves :: "itrm \<Rightarrow> nat"
 where
     "rleaves (Pure _) = 0"
-  | "rleaves (Imp _)  = 1"
+  | "rleaves (Term _)  = 1"
   | "rleaves (f \<diamond> x)  = rleaves f + leaves x"
 
 lemma min_leaves: "0 < leaves x"
@@ -39,27 +335,89 @@ by induction auto
 
 subsection {* Normal form *}
 
-inductive_set NF :: "'a itrm set"
+inductive_set NF :: "itrm set"
 where
-    pure_nf[intro]: "Pure x \<in> NF"
-  | ap_nf[intro]:   "f \<in> NF \<Longrightarrow> f \<diamond> Imp x \<in> NF"
+    pure_nf[simp,intro]: "Pure x \<in> NF"
+  | ap_nf[intro]:   "f \<in> NF \<Longrightarrow> f \<diamond> Term x \<in> NF"
+
+fun NF_head :: "itrm \<Rightarrow> dB"
+where
+    "NF_head (Pure x) = x"
+  | "NF_head (f \<diamond> x) = NF_head f"
 
 lemma ap_nfD1[dest]: "f \<diamond> x \<in> NF \<Longrightarrow> f \<in> NF"
 by (rule NF.cases) auto
 
-lemma ap_nfD2[dest]: "f \<diamond> x \<in> NF \<Longrightarrow> \<exists>x'. x = Imp x'"
+lemma ap_nfD2[dest]: "f \<diamond> x \<in> NF \<Longrightarrow> \<exists>x'. x = Term x'"
 by (rule NF.cases) auto
 
-lemma imp_not_nf[dest]: "Imp x \<in> NF \<Longrightarrow> False"
+lemma term_not_nf[dest]: "Term x \<in> NF \<Longrightarrow> False"
 by (rule NF.cases) auto
+
+lemma nf_cong:
+  assumes "n \<in> NF" "n' \<in> NF"
+      and "opaque n = opaque n'"
+      and "NF_head n \<leftrightarrow> NF_head n'"
+    shows "n \<cong> n'"
+using assms proof (induction arbitrary: n')
+  case (pure_nf x)
+    then obtain y where "n' = Pure y" by cases auto
+    with pure_nf.prems show ?case by (auto intro: itrm_cong.intros)
+next
+  case (ap_nf f x)
+    note `n' \<in> NF` and `opaque (f \<diamond> Term x) = opaque n'`
+    then obtain g y where n'_split: "n' = g \<diamond> Term y" "g \<in> NF"
+      by cases auto
+    with ap_nf.prems have "opaque f = opaque g" "NF_head f \<leftrightarrow> NF_head g" by auto
+    with ap_nf.IH `g \<in> NF` have "f \<cong> g" by simp
+    with ap_nf.prems n'_split show ?case by (auto intro: itrm_cong.intros)
+qed
+
+lemma nf_unlift:
+  assumes "n \<in> NF"
+    shows "NF_head n \<leftrightarrow> unlift n"
+using assms proof (induction set: NF)
+  case (pure_nf x)
+  show ?case by simp
+next
+  case (ap_nf f x)
+  let ?n = "iorder f + 1"
+  have "unlift (f \<diamond> Term x) = wrap_abs (unlift' ?n f 1 \<degree> Var 0) ?n"
+    unfolding unlift_ap by simp
+  also have "... = wrap_abs (Abs (unlift' ?n f 1 \<degree> Var 0)) (iorder f)"
+    using wrap_abs_inside by simp
+  also have "... \<leftrightarrow> unlift f" proof -
+    have "\<not> free (unlift' ?n f 1) 0" using free_unlift by fastforce
+    hence "Abs (unlift' ?n f 1 \<degree> Var 0) \<rightarrow>\<^sub>\<eta> (unlift' ?n f 1)[Var 0/0]" ..
+    also have "... = unlift' (iorder f) f 0"
+      using unlift_subst by (metis One_nat_def Suc_eq_plus1 le0)
+    finally show ?thesis
+      by (simp add: r_into_rtranclp wrap_abs_equiv beta_eta_red)
+  qed
+  finally show ?case
+    using NF_head.simps ap_nf.IH term_sym term_trans by presburger
+qed
+
+lemma nf_unique:
+  assumes in_nf: "n \<in> NF" "n' \<in> NF"
+      and equiv: "n \<simeq> n'"
+    shows "n \<cong> n'"
+using in_nf proof (rule nf_cong)
+  from equiv show "opaque n = opaque n'" by (rule opaque_equiv)
+  from equiv have "unlift n \<leftrightarrow> unlift n'" by (rule unlift_equiv)
+  thus "NF_head n \<leftrightarrow> NF_head n'"
+    using nf_unlift[OF in_nf(1)] nf_unlift[OF in_nf(2)]
+    using term_sym term_trans
+    by presburger
+qed
 
 
 subsection {* Normalization of idiomatic terms *}
 
-function (sequential) normalize_pure_nf :: "'a itrm \<Rightarrow> 'a itrm"
+function (sequential) normalize_pure_nf :: "itrm \<Rightarrow> itrm"
 where
-    "normalize_pure_nf (Pure g \<diamond> (f \<diamond> x)) = normalize_pure_nf (Pure (\<B>\<^sub>1 g) \<diamond> f) \<diamond> x"
-  | "normalize_pure_nf (Pure f \<diamond> Pure x) = Pure (f $ x)"
+    "normalize_pure_nf (Pure g \<diamond> (f \<diamond> x)) = normalize_pure_nf (Pure (\<B> \<degree> g) \<diamond> f) \<diamond> x"
+  | "normalize_pure_nf (Pure f \<diamond> Pure x) = Pure (f \<degree> x)"
   | "normalize_pure_nf x = x"
 by pat_completeness auto
 termination by (relation "measure (\<lambda>t.
@@ -70,27 +428,27 @@ termination by (relation "measure (\<lambda>t.
 lemma pure_nf_rleaves: "rleaves (normalize_pure_nf (Pure f \<diamond> x)) \<le> rleaves x"
 by (induct "Pure f \<diamond> x" arbitrary: f x rule: normalize_pure_nf.induct) auto
 
-fun normalize_nf_pure :: "'a itrm \<Rightarrow> 'a itrm"
+fun normalize_nf_pure :: "itrm \<Rightarrow> itrm"
 where
-    "normalize_nf_pure (f \<diamond> Pure x) = normalize_pure_nf (Pure (Abs (BVar 0 $ x)) \<diamond> f)"
+    "normalize_nf_pure (f \<diamond> Pure x) = normalize_pure_nf (Pure (\<A>' \<degree> x) \<diamond> f)"
   | "normalize_nf_pure x = x"
 
-function (sequential) normalize_nf_nf :: "'a itrm \<Rightarrow> 'a itrm"
+function (sequential) normalize_nf_nf :: "itrm \<Rightarrow> itrm"
 where
     "normalize_nf_nf (g \<diamond> (f \<diamond> x)) = normalize_nf_nf (normalize_pure_nf (Pure \<B> \<diamond> g) \<diamond> f) \<diamond> x"
   | "normalize_nf_nf x = normalize_nf_pure x"
 by pat_completeness auto
 termination proof
-  fix g f x :: "'a itrm"
+  fix g f x
   have "rleaves (normalize_pure_nf (Pure \<B> \<diamond> g)) \<le> rleaves g" using pure_nf_rleaves .
   also have "rleaves g < rleaves g + leaves x" using min_leaves by simp
   finally show "(normalize_pure_nf (Pure \<B> \<diamond> g) \<diamond> f, g \<diamond> (f \<diamond> x)) \<in> measure rleaves" by simp
 qed simp
 
-fun normalize :: "'a itrm \<Rightarrow> 'a itrm"
+fun normalize :: "itrm \<Rightarrow> itrm"
 where
     "normalize (Pure x) = Pure x"
-  | "normalize (Imp x)  = Pure (Abs (BVar 0)) \<diamond> Imp x"
+  | "normalize (Term x)  = Pure \<I> \<diamond> Term x"
   | "normalize (x \<diamond> y)  = normalize_nf_nf (normalize x \<diamond> normalize y)"
 
 
@@ -110,10 +468,12 @@ lemma nf_nf_in_nf:
   assumes "x \<in> NF" and "f \<in> NF"
     shows "normalize_nf_nf (f \<diamond> x) \<in> NF"
 using assms
-by (induction arbitrary: f rule: NF.induct) (auto intro: pure_nf_in_nf nf_pure_in_nf)
+by (induction arbitrary: f rule: NF.induct) (auto intro: pure_nf_in_nf)
 
 lemma normalized: "normalize x \<in> NF"
 by (induction x rule: normalize.induct) (auto intro: nf_nf_in_nf)
+
+(* TODO normalize x \<simeq> x *)
 
 
 end
